src/Spec/Hoare.v
@@ -13,30 +13,27 @@ Record SpecProps T R State :=
     post: State -> T -> Prop;
     alternate: State -> R -> Prop; }.
 
-Definition Specification A T R State := A -> State -> SpecProps T R State.
+Definition Specification T R State := State -> SpecProps T R State.
 
-Definition spec_exec A T R State (spec: Specification A T R State) :
+Definition spec_exec T R State (spec: Specification T R State) :
   relation State State T :=
-  fun s s' r => forall a,
-    (spec a s).(pre) -> (spec a s).(post) s' r.
+  fun s s' r => (spec s).(pre) -> (spec s).(post) s' r.
 
-Definition spec_aexec A T R State (spec: Specification A T R State) :
+Definition spec_aexec T R State (spec: Specification T R State) :
   relation State State R :=
-  fun s s' r => forall a,
-    (spec a s).(pre) -> (spec a s).(alternate) s' r.
+  fun s s' r => (spec s).(pre) -> (spec s).(alternate) s' r.
 
-Definition spec_impl A A'
-           `(spec1: Specification A' T R State)
-           `(spec2: Specification A T R State) :=
-  forall a s, (spec2 a s).(pre) ->
-         exists a', (spec1 a' s).(pre) /\
-               (forall s' v, (spec1 a' s).(post) s' v ->
-                        (spec2 a s).(post) s' v) /\
-               (forall s' rv, (spec1 a' s).(alternate) s' rv ->
-                         (spec2 a s).(alternate) s' rv).
+Definition spec_impl
+           `(spec1: Specification T R State)
+           `(spec2: Specification T R State) :=
+  forall s, (spec2 s).(pre) -> (spec1 s).(pre) /\
+            (forall s' v, (spec1 s).(post) s' v ->
+                          (spec2 s).(post) s' v) /\
+            (forall s' rv, (spec1 s).(alternate) s' rv ->
+                           (spec2 s).(alternate) s' rv).
 
-Definition op_spec `(sem: Dynamics Op State) `(op : Op T) : Specification unit T unit State :=
-  fun (_:unit) state =>
+Definition op_spec `(sem: Dynamics Op State) `(op : Op T) : Specification T unit State :=
+  fun state =>
     {|
       pre := True;
       post :=
@@ -55,56 +52,56 @@ Section Hoare.
   Notation crash_step := sem.(crash_step).
   Notation rexec := sem.(rexec).
 
-  Definition proc_rspec A T R
+  Definition proc_rspec T R
              (p: proc T) (rec: proc R)
-             (spec: Specification A T R State) :=
+             (spec: Specification T R State) :=
     exec p ---> spec_exec spec /\
     rexec p rec ---> spec_aexec spec.
 
-  Definition proc_cspec A T
+  Definition proc_cspec T
              (p: proc T)
-             (spec: Specification A T unit State) :=
+             (spec: Specification T unit State) :=
     exec p ---> spec_exec spec /\
     exec_crash p ---> spec_aexec spec.
 
-  Theorem proc_rspec_expand A T R
+  Theorem proc_rspec_expand T R
           (p: proc T) (rec: proc R)
-          (spec: Specification A T R State) :
+          (spec: Specification T R State) :
     proc_rspec p rec spec <->
-    forall a s,
-      (spec a s).(pre) ->
+    forall s,
+      (spec s).(pre) ->
       (forall s' v, exec p s s' v ->
-               (spec a s).(post) s' v) /\
+               (spec s).(post) s' v) /\
       (forall s' rv, rexec p rec s s' rv ->
-                (spec a s).(alternate) s' rv).
+                (spec s).(alternate) s' rv).
   Proof.
     unfold proc_rspec, rimpl, spec_exec, spec_aexec; split; intros.
     - intuition eauto 10.
-    - split; intros.
-      specialize (H a x); intuition eauto.
-      specialize (H a x); intuition eauto.
+    - split; intros x y ?.
+      specialize (H x); intuition eauto.
+      specialize (H x); intuition eauto.
   Qed.
 
-  Theorem proc_cspec_expand A T (p: proc T)
-          (spec: Specification A T unit State) :
+  Theorem proc_cspec_expand T (p: proc T)
+          (spec: Specification T unit State) :
     proc_cspec p spec <->
-    forall a s,
-      (spec a s).(pre) ->
+    forall s,
+      (spec s).(pre) ->
       (forall s' v, exec p s s' v ->
-               (spec a s).(post) s' v) /\
+               (spec s).(post) s' v) /\
       (forall s' rv, exec_crash p s s' rv ->
-                (spec a s).(alternate) s' rv).
+                (spec s).(alternate) s' rv).
   Proof.
     unfold proc_cspec, rimpl, spec_exec, spec_aexec; split; intros.
     - intuition eauto 10.
-    - split; intros.
-      specialize (H a x); intuition eauto.
-      specialize (H a x); intuition eauto.
+    - split; intros x y ?.
+      specialize (H x); intuition eauto.
+      specialize (H x); intuition eauto.
   Qed.
 
-  Theorem proc_rspec_impl A A'
-          `(spec1: Specification A' T R State)
-          `(spec2: Specification A T R State)
+  Theorem proc_rspec_impl
+          `(spec1: Specification T R State)
+          `(spec2: Specification T R State)
           p rec :
     spec_impl spec1 spec2 ->
     proc_rspec p rec spec1 ->
@@ -113,14 +110,14 @@ Section Hoare.
     unfold spec_impl; intros.
     pose proof (proj1 (proc_rspec_expand _ _ _) H0); clear H0.
     apply proc_rspec_expand; intros.
-    specialize (H a s); propositional.
-    specialize (H1 a' s); propositional.
+    specialize (H s); propositional.
+    specialize (H1 s); propositional.
     eauto 10.
   Qed.
 
-  Theorem proc_cspec_impl A A'
-          `(spec1: Specification A' T unit State)
-          `(spec2: Specification A T unit State)
+  Theorem proc_cspec_impl
+          `(spec1: Specification T unit State)
+          `(spec2: Specification T unit State)
           p :
     spec_impl spec1 spec2 ->
     proc_cspec p spec1 ->
@@ -129,106 +126,102 @@ Section Hoare.
     unfold spec_impl; intros.
     pose proof (proj1 (proc_cspec_expand _ _) H0); clear H0.
     apply proc_cspec_expand; intros.
-    specialize (H a s); propositional.
-    specialize (H1 a' s); propositional.
-    eauto 10.
+    firstorder.
   Qed.
 
-  Theorem proc_rspec_exec_equiv A T `(spec: Specification A T R State)
+  Theorem proc_rspec_exec_equiv T `(spec: Specification T R State)
           (p p': proc T) `(rec: proc R):
       exec_equiv sem p p' ->
       proc_rspec p' rec spec ->
       proc_rspec p rec spec.
   Proof. unfold proc_rspec. intros ->; auto. Qed.
 
-  Theorem proc_cspec_exec_equiv A T `(spec: Specification A T unit State)
+  Theorem proc_cspec_exec_equiv T `(spec: Specification T unit State)
           (p p': proc T):
       exec_equiv sem p p' ->
       proc_cspec p' spec ->
       proc_cspec p spec.
   Proof. unfold proc_cspec. intros ->; auto. Qed.
 
-  Theorem proc_rspec_rx A T A' T' R `(spec: Specification A T R State)
+  Theorem proc_rspec_rx T T' R `(spec: Specification T R State)
                            `(p: proc T) `(rec: proc R)
                            `(rx: T -> proc T')
-                           `(spec': Specification A' T' R State):
+                           `(spec': Specification T' R State):
       proc_rspec p rec spec ->
-      (forall a' state, pre (spec' a' state) ->
-               exists a, pre (spec a state) /\
+      (forall state, pre (spec' state) -> pre (spec state) /\
                     (forall r,
                         proc_rspec (rx r) rec
-                          (fun (_:unit) state' =>
-                             {| pre := post (spec a state) state' r;
+                          (fun state' =>
+                             {| pre := post (spec state) state' r;
                                 post :=
                                   fun (state'' : State) r =>
-                                    post (spec' a' state) state'' r;
+                                    post (spec' state) state'' r;
                                 alternate :=
                                   fun (state'' : State) r =>
-                                    alternate (spec' a' state) state'' r |})
+                                    alternate (spec' state) state'' r |})
                     ) /\
-                    (forall (r: R) (state': State), alternate (spec a state) state' r ->
-                             alternate (spec' a' state) state' r)) ->
+                    (forall (r: R) (state': State), alternate (spec state) state' r ->
+                             alternate (spec' state) state' r)) ->
       proc_rspec (Bind p rx) rec spec'.
   Proof.
     unfold proc_rspec at 3. intros (Hp_ok&Hp_rec) Hrx.
     split.
     - simpl; rew Hp_ok.
-      intros state state' t' (t&(state_mid&Hspec_mid&Hexec_mid)) a' Hpre'.
-      specialize (Hrx _ _ Hpre') as (a&Hpre&Hok&Hrec).
+      intros state state' t' (t&(state_mid&Hspec_mid&Hexec_mid)) Hpre'.
+      specialize (Hrx _ Hpre') as (Hpre&Hok&Hrec).
       specialize (Hok t). rewrite proc_rspec_expand in Hok.
-      destruct (Hok tt state_mid) as (Hrx_ok&Hrx_rec); simpl; eauto.
+      destruct (Hok state_mid) as (Hrx_ok&Hrx_rec); simpl; eauto.
     - rewrite rexec_unfold. rewrite rexec_unfold in Hp_rec.
       simpl. rewrite exec_crash_idem, bind_dist_r.
       apply rel_or_elim.
       + rewrite Hp_rec; auto.
-        intros state state' r Hspec_aexec a' Hpre'.
-        specialize (Hrx _ _ Hpre') as (a&Hpre&?&Hrec); eauto.
+        intros state state' r Hspec_aexec Hpre'.
+        specialize (Hrx _ Hpre') as (Hpre&?&Hrec); eauto.
       + rewrite bind_assoc, Hp_ok.
-        intros state state' t' (t&(state_mid&Hspec_mid&Hcrash_mid)) a' Hpre'.
-      specialize (Hrx _ _ Hpre') as (a&Hpre&Hok&Hrec).
+        intros state state' t' (t&(state_mid&Hspec_mid&Hcrash_mid)) Hpre'.
+      specialize (Hrx _ Hpre') as (Hpre&Hok&Hrec).
       specialize (Hok t). rewrite proc_rspec_expand in Hok.
-      destruct (Hok tt state_mid) as (Hrx_ok&Hrx_rec); simpl; eauto.
+      destruct (Hok state_mid) as (Hrx_ok&Hrx_rec); simpl; eauto.
   Qed.
 
-  Theorem proc_cspec_rx A T A' T' `(spec: Specification A T unit State)
+  Theorem proc_cspec_rx T T' `(spec: Specification T unit State)
                            `(p: proc T)
                            `(rx: T -> proc T')
-                           `(spec': Specification A' T' unit State):
+                           `(spec': Specification T' unit State):
       proc_cspec p spec ->
-      (forall a' state, pre (spec' a' state) ->
-               exists a, pre (spec a state) /\
+      (forall state, pre (spec' state) -> pre (spec state) /\
                     (forall r,
                         proc_cspec (rx r)
-                          (fun (_:unit) state' =>
-                             {| pre := post (spec a state) state' r;
+                          (fun state' =>
+                             {| pre := post (spec state) state' r;
                                 post :=
                                   fun (state'' : State) r =>
-                                    post (spec' a' state) state'' r;
+                                    post (spec' state) state'' r;
                                 alternate :=
                                   fun (state'' : State) r =>
-                                    alternate (spec' a' state) state'' r |})
+                                    alternate (spec' state) state'' r |})
                     ) /\
-                    (forall (r:  unit) (state': State), alternate (spec a state) state' r ->
-                             alternate (spec' a' state) state' r)) ->
+                    (forall (r:  unit) (state': State), alternate (spec state) state' r ->
+                             alternate (spec' state) state' r)) ->
       proc_cspec (Bind p rx) spec'.
   Proof.
     unfold proc_cspec at 3. intros (Hp_ok&Hp_rec) Hrx.
     split.
     - simpl; rew Hp_ok.
-      intros state state' t' (t&(state_mid&Hspec_mid&Hexec_mid)) a' Hpre'.
-      specialize (Hrx _ _ Hpre') as (a&Hpre&Hok&Hrec).
+      intros state state' t' (t&(state_mid&Hspec_mid&Hexec_mid)) Hpre'.
+      specialize (Hrx _ Hpre') as (Hpre&Hok&Hrec).
       specialize (Hok t). rewrite proc_cspec_expand in Hok.
-      destruct (Hok tt state_mid) as (Hrx_ok&Hrx_rec); simpl; eauto.
+      destruct (Hok state_mid) as (Hrx_ok&Hrx_rec); simpl; eauto.
     - simpl. rewrite exec_crash_idem.
       apply rel_or_elim.
       + rewrite Hp_rec; auto.
-        intros state state' r Hspec_aexec a' Hpre'.
-        specialize (Hrx _ _ Hpre') as (a&Hpre&?&Hrec); eauto.
+        intros state state' r Hspec_aexec Hpre'.
+        specialize (Hrx _ Hpre') as (Hpre&?&Hrec); eauto.
       + rewrite Hp_ok.
-        intros state state' t' (t&(state_mid&Hspec_mid&Hcrash_mid)) a' Hpre'.
-        specialize (Hrx _ _ Hpre') as (a&Hpre&Hok&Hrec).
+        intros state state' t' (t&(state_mid&Hspec_mid&Hcrash_mid)) Hpre'.
+        specialize (Hrx _ Hpre') as (Hpre&Hok&Hrec).
         specialize (Hok t). rewrite proc_cspec_expand in Hok.
-        destruct (Hok tt state_mid) as (Hrx_ok&Hrx_rec); simpl; eauto.
+        destruct (Hok state_mid) as (Hrx_ok&Hrx_rec); simpl; eauto.
   Qed.
 
   (** ** Reasoning about the [Ret] return operation.
@@ -253,7 +246,7 @@ Section Hoare.
     forall T (v:T),
       proc_rspec
         (Ret v) rec
-        (fun (_:unit) state =>
+        (fun state =>
            {| pre := True;
               post := fun state' r => r = v /\
                                       state' = state;
@@ -268,42 +261,38 @@ Section Hoare.
     [spec] matches the [wipe] relation:
    *)
 
-  Theorem ret_rspec A T R (wipe: State -> State -> Prop) `(spec: Specification A T R State)
+  Theorem ret_rspec T R (wipe: State -> State -> Prop) `(spec: Specification T R State)
           (v:T) (rec: proc R):
     rec_noop rec wipe ->
-    (forall a state, pre (spec a state) ->
-                     post (spec a state) state v /\
+    (forall state, pre (spec state) ->
+                     post (spec state) state v /\
                      forall state', wipe state state' ->
-                                    forall (r : R), alternate (spec a state) state' r) ->
+                                    forall (r : R), alternate (spec state) state' r) ->
     proc_rspec (Ret v) rec spec .
   Proof.
     unfold proc_rspec; intros Hnoop Himpl; split.
-    - intros state state' t Hexec a Hpre.
-      inversion Hexec; subst. specialize (Himpl _ _ Hpre). intuition.
+    - intros state state' t Hexec Hpre.
+      inversion Hexec; subst. specialize (Himpl _ Hpre). intuition.
     - destruct (Hnoop _ v) as (?&->).
-      unfold spec_aexec.
-      intros s s' r Hl a Hpre. specialize (Hl tt).
-      eapply Himpl; eauto.
-      eapply Hl; simpl; eauto.
+      unfold spec_aexec. firstorder.
   Qed.
 
-  Theorem ret_cspec A T `(spec: Specification A T unit State)
+  Theorem ret_cspec T `(spec: Specification T unit State)
           (v:T):
-    (forall a state, pre (spec a state) ->
-                     post (spec a state) state v /\
-                     alternate (spec a state) state tt) ->
+    (forall state, pre (spec state) ->
+                     post (spec state) state v /\
+                     alternate (spec state) state tt) ->
     proc_cspec (Ret v) spec .
   Proof.
     unfold proc_cspec; intros Himpl; split;
-    intros state state' t Hexec a Hpre;
-    inversion Hexec; subst; specialize (Himpl _ _ Hpre); intuition.
+    intros state state' t Hexec Hpre;
+    inversion Hexec; subst; specialize (Himpl _ Hpre); intuition.
   Qed.
 
   (** Define what it means for a spec to be idempotent: *)
-  Definition idempotent A T R `(spec: Specification A T R State) :=
-    forall a state,
-      pre (spec a state) ->
-      forall v state', alternate (spec a state) state' v ->
+  Definition idempotent A T R `(spec: A -> Specification T R State) :=
+    forall a state, pre (spec a state) ->
+      forall v state', alternate (spec a state) state' v -> 
               (** idempotency: alternate condition implies precondition to
                  re-run on every crash *)
               exists a', pre (spec a' state') /\
@@ -314,87 +303,14 @@ Section Hoare.
                     forall rv state'', post (spec a' state') state'' rv ->
                                   post (spec a state) state'' rv.
 
-  Definition idempotent_crash_step A T R `(spec: Specification A T R State) :=
+  Definition idempotent_crash_step A T R `(spec: A -> Specification T R State) :=
     forall a state,
       pre (spec a state) ->
       forall v state' state'', alternate (spec a state) state' v ->
                                crash_step state' state'' tt ->
-              exists a', pre (spec a' state'') /\
+               exists a', pre (spec a' state'') /\
                     forall rv state''', post (spec a' state'') state''' rv ->
                                   post (spec a state) state''' rv.
-
-  (*
-  (* Idempotents theorem: *)
-  Theorem idempotent_loopspec A `(rec: proc unit) `(rec': proc unit)
-        `(spec: Specification A unit unit State)
-        (Hspec: proc_rspec rec' rec spec):
-        idempotent spec ->
-        proc_loopspec rec' rec spec.
-  Proof.
-    unfold proc_loopspec; intros.
-    destruct Hspec as (Hse&Hsr).
-    rew Hsr.
-    Split.
-    - auto.
-    - rew Hse.
-      intros s s'' tt Hrs a Hpre.
-      inversion Hrs as ([]&s'&Hrs'&?).
-      specialize (Hrs' a Hpre). unfold idempotent in H.
-      edestruct H as (a'&Hpre'&Hpost); eauto.
-  Qed.
-   *)
-
-  (*
-  Theorem compose_recovery A A' A'' `(spec: Specification A'' T unit State)
-                               `(rspec: Specification A' unit unit State)
-                               `(spec': Specification A T unit State)
-                               `(p: proc T) `(rec: proc unit) `(rec': proc unit)
-        (Hspec: proc_rspec p rec spec)
-        (Hrspec: proc_loopspec rec' rec rspec)
-        (Hspec_spec':
-           forall (a:A) state, pre (spec' a state) ->
-                      exists (a'':A''),
-                        pre (spec a'' state) /\
-                        (forall v state', post (spec a'' state) v state' ->
-                                 post (spec' a state) v state') /\
-                        (forall v state', alternate (spec a'' state) state' v ->
-                                 exists a', pre (rspec a' state') /\
-                                       forall v' state'',
-                                         post (rspec a' state') state'' v' ->
-                                         alternate (spec' a state) state'' v')):
-        proc_rspec p (Bind rec (fun _ => rec')) spec'.
-  Proof.
-    unfold proc_rspec; intros; split.
-    - destruct Hspec as (->&?).
-      intros s s' t Hspec a Hpre.
-      edestruct Hspec_spec' as (a''&?&Hp&?); eauto.
-    - unfold rexec; simpl. unfold exec_recover; simpl.
-      unfold proc_loopspec in Hrspec.
-      unfold rexec in Hrspec. unfold exec_recover in Hrspec.
-      destruct Hspec as (?&Hrec).
-      unfold rexec in Hrec. unfold exec_recover in Hrec.
-      repeat setoid_rewrite bind_dist_r; norm.
-
-      (* Base case *)
-      assert (_ <- exec_crash sem p;
-              _ <- sem.(crash_step);
-              _ <- exec rec;
-              exec rec'
-                   --->
-                   spec_aexec spec').
-      { rew <- seq_star_none in Hrec.
-        rew <- rel_or_introl in Hrspec.
-        rew Hrspec.
-        left_assoc rew Hrec.
-        intros s1 s3 [] Hl a Hpre.
-        destruct Hl as ([]&s2&Hrexec_spec&?Hexec_rspec).
-        edestruct Hspec_spec' as (?&?&?&Hrec'); eauto.
-        edestruct Hrec'.
-        { eapply Hrexec_spec; eauto. }
-        destruct H2 as (?&?). eapply H3. eapply Hexec_rspec. eauto.
-      }
-  Abort.
-   *)
 
   (** In some situations, the precondition of a specification
     may define variables or facts that you want to [intros].
@@ -405,40 +321,40 @@ Section Hoare.
     arbitrary Prop in question as a hypothesis about [state0].
   *)
 
-  Theorem rspec_intros A T R `(spec: Specification A T R State)
+  Theorem rspec_intros T R `(spec: Specification T R State)
           `(p: proc T) `(rec: proc R):
-      (forall a state0,
-          pre (spec a state0) ->
+      (forall state0,
+          pre (spec state0) ->
           proc_rspec p rec
-            (fun (_:unit) state =>
+            (fun state =>
                {| pre := state = state0;
                   post :=
-                    fun state' r => post (spec a state) state' r;
+                    fun state' r => post (spec state) state' r;
                   alternate :=
-                    fun state' r => alternate (spec a state) state' r;
+                    fun state' r => alternate (spec state) state' r;
                |})) ->
       proc_rspec p rec spec.
   Proof.
     unfold proc_rspec at 2; intros H.
-    split; intros s s' r Hexec a Hpre; eapply H; simpl; eauto using tt.
+    split; intros s s' r Hexec Hpre; eapply H; simpl; eauto.
   Qed.
 
-  Theorem cspec_intros A T `(spec: Specification A T unit State)
+  Theorem cspec_intros T `(spec: Specification T unit State)
           `(p: proc T):
-      (forall a state0,
-          pre (spec a state0) ->
+      (forall state0,
+          pre (spec state0) ->
           proc_cspec p
-            (fun (_:unit) state =>
+            (fun state =>
                {| pre := state = state0;
                   post :=
-                    fun state' r => post (spec a state) state' r;
+                    fun state' r => post (spec state) state' r;
                   alternate :=
-                    fun state' r => alternate (spec a state) state' r;
+                    fun state' r => alternate (spec state) state' r;
                |})) ->
       proc_cspec p spec.
   Proof.
     unfold proc_cspec at 2; intros H.
-    split; intros s s' r Hexec a Hpre; eapply H; simpl; eauto using tt.
+    split; intros s s' r Hexec Hpre; eapply H; simpl; eauto using tt.
   Qed.
 
   (*
@@ -467,15 +383,16 @@ Section Hoare.
     proc_cspec (Prim op) (op_spec sem op).
   Proof.
     unfold proc_cspec; split.
-    - intros state state' t Hexec a Hpre; eauto.
+    - intros state state' t Hexec Hpre; eauto.
     - simpl. apply rel_or_elim.
-      * intros s s' [] Hl a Hpre. simpl. split; auto.
+      * intros s s' [] Hl Hpre. simpl. split; auto.
         firstorder.
-      * intros s s' [] Hl a Hpre.
+      * intros s s' [] Hl Hpre.
         inversion Hl as (?&?&?&Hrest). inversion Hrest; subst.
         firstorder.
   Qed.
 
+  (*
   Theorem proc_cspec_to_rspec A A' T R (cspec: Specification A T unit State)
           `(rec_cspec: Specification A' R unit State)
           `(rspec: Specification A' T R State)
@@ -527,6 +444,7 @@ Section Hoare.
          admit.
       }
    Abort.
+   *)
 
 
 End Hoare.
